feat: introduce restrictions on `include`s and `open`s
This commit introduces the following syntaxes:
```fstar
// brings `MyModule.some_function`, `MyModule.some_type` and `MyModule.SomeConstructor` only, nothing else is visible
open MyModule { some_function, some_type, SomeConstructor }
// `include` works the same
include MyModule { some_function, some_type, SomeConstructor }
// renaming is possible
include MyModule { some_function as f, SomeConstructor as X }
```

I call `{ ... }` a restriction that we impose on the open or include, maybe there's a better naming there.

This PR:
 - tags auto generated records (when `type foo = | Foo {...}`) with a new attribute `desugar_of_variant_record` (this is important, so that `open Module {foo}` is able to look for that attribute and bring `foo__Foo__payload` in scope too);
 - add a type `restriction`;
 - change the parser to allow the new restriction syntax;
 - tweaks `DsEnv` accordingly.

src/syntax/FStar.Syntax.Syntax.fsti
@@ -645,7 +645,16 @@ type open_kind =                                          (* matters only for re
 | Open_module                                             (* only opens the module, not the namespace *)
 | Open_namespace  
 
-type open_module_or_namespace = (lident & open_kind)      (* lident fully qualified name, already resolved. *)
+type ident_alias = option ident
+
+(** A restriction imposed on a `open` or `include` declaration. *)
+type restriction = 
+     (** No restriction, the entire module is opened or included. *)
+     | Unrestricted
+     (** Only a specific subset of the exported definition of a module is opened or included. *)
+     | AllowList of list (ident & ident_alias)
+
+type open_module_or_namespace = (lident & open_kind & restriction)      (* lident fully qualified name, already resolved. *)
 type module_abbrev = (ident & lident)                     (* module X = A.B.C, where A.B.C is fully qualified and already resolved *)
 
 (*
@@ -894,6 +903,19 @@ val t_erased_of     : term -> term
 
 val unit_const_with_range : Range.range -> term
 val unit_const            : term
+
+(** Checks wether an identity `id` is allowed by a include/open
+restriction `r`. If it is not allowed,
+`is_ident_allowed_by_restriction id r` returns `None`, otherwise it
+returns `Some renamed`, where `renamed` is either `id` (when no there
+is no `as` clause) or another identity pointing to the actual source
+identity in the source module.
+
+For example, if we have `open Foo { my_type as the_type }`,
+`is_ident_allowed_by_restriction <the_type> <{ my_type as the_type }>`
+will return `Some <my_type>`.
+*)
+val is_ident_allowed_by_restriction: ident -> restriction -> option ident
 
 instance val has_range_syntax #a : unit -> Tot (hasRange (syntax a))
 instance val has_range_withinfo #a : unit -> Tot (hasRange (withinfo_t a))
